Extraction to C examples for poly1305 and Chacha20

examples/low-star/fstarlib.h
@@ -1,7 +1,0 @@
-typedef int Prims_bool;
-
-typedef struct{int x; int y;} intint_tuple;
-typedef struct{char x; char y;} charchar_tuple;
-
-
-int parse_int(char *string);
