examples/stateful_bignum/bignum.fst
@@ -1,9 +1,0 @@
-module Bignum
-
-let add = Addition.addition_with_lemma
-let smul = ScalarMultiplication.scalar_multiplication_with_lemma
-let mul = Multiplication.multiplication
-let copy = Bigint.copy
-let shift = Shift.shift
-let carry = Carry.carry
-let retemplate = Retemplate.retemplate
