examples/primitives/FStar.SBytes.fst
@@ -1,0 +1,56 @@
+(*--build-config
+  options:--admit_fsi FStar.Set --verify_module Buffer32;
+  other-files:FStar.Classical.fst FStar.PredicateExtensionality.fst FStar.Set.fsi seq.fsi FStar.Seq.fst FStar.SeqProperties.fst FStar.Heap.fst FStar.ST.fst FStar.All.fst FStar.Array.fst FStar.Ghost.fst axioms.fst intlib.fst sint.fst FStar.UInt8.fst sbuffer.fst;
+  --*)
+
+module FStar.SBytes
+
+open FStar.Ghost
+open FStar.Heap
+open IntLib
+open Sint
+open FStar.UInt8
+open FStar.UInt32
+open SBuffer
+
+(* Contains coercion functions between integers and bytes that can be optimized in low-level code *)
+
+type sbytes = buffer 8
+type uint32 = usint 32
+
+(**)
+let create = create #8
+let index = index #8
+let upd = upd #8
+let sub = sub #8
+let blit = blit #8
+let split = split #8
+let copy = copy #8
+let offset = offset #8
+(**)
+
+opaque type Equals (ha:heap) (a:buffer 32) (hb:heap) (b:sbytes) (l:nat) =
+  l <= length a /\ 4 * l <= length b /\ Live ha a /\ Live hb b 
+  /\ (forall (i:nat). {:pattern (get ha a i) \/ get hb b (4*i+0) \/ get hb b (4*i+0) \/ get hb b (4*i+0) } 
+       i < l ==> v (get ha a i) = v (get hb b (4*i+0)) + pow2 8 * v (get hb b (4*i+1)) +
+		         pow2 16 * v (get hb b (4*i+2)) + pow2 24 * v (get hb b (4*i+3)))
+
+assume val uint32_of_sbytes: b:sbytes{length b >= 4} -> ST uint32
+  (requires (fun h -> Live h b))
+  (ensures (fun h0 r h1 -> Live h0 b /\ h0 == h1 
+			 /\ v r = v (get h0 b 0) + pow2 8 * v (get h0 b 1) +
+			         pow2 16 * v (get h0 b 2) + pow2 24 * v (get h0 b 3)))
+
+assume val sbytes_of_uint32s: res:sbytes -> b:buffer 32{Disjoint res b} -> l:nat{l<=length b /\ 4*l <= length res} -> ST unit
+  (requires (fun h -> Live h res /\ Live h b))
+  (ensures (fun h0 _ h1 -> Equals h0 b h1 res l /\ Modifies (only res) h0 h1))
+
+(* TODO : do something to make sure that if output is a or b it still works *)
+assume val xor_bytes: output:sbytes -> a:sbytes -> b:sbytes{Disjoint a b} -> l:nat{l <= length b /\ l <= length a /\ l <= length output} -> ST unit
+  (requires (fun h -> Live h output /\ Live h a /\ Live h b))
+  (ensures (fun h0 _ h1 -> Live h0 a /\ Live h0 b /\ Live h1 output /\ Modifies (only output) h0 h1
+    /\ (forall (i:nat). {:pattern (get h1 output i)} i < l ==> 
+      v (get h1 output i) = v (FStar.UInt8.logxor (get h0 a i) (get h0 b i))) ))
+
+assume val print: sbytes -> Tot unit
+assume val print_bytes: sbytes -> Tot unit
