examples/primitives/FStar.UInt64.fst
@@ -1,0 +1,67 @@
+(*--build-config
+  options:--verify_module FStar.UInt64;
+  other-files:FStar.Ghost.fst axioms.fst intlib.fst sint.fst;
+  --*)
+
+module FStar.UInt64
+
+open FStar.Ghost
+open IntLib
+open Sint
+
+assume val n: x:pos{x = 64}
+
+type uint64 = usint n
+type uint128 = usint (2*n)
+
+let (zero:uint64) = uzero n
+let (one:uint64) = uone n
+let (ones:uint64) = uones n
+
+let (max_int:erased nat) = eumax_int #n
+let (min_int:erased nat) = eumin_int #n
+
+let (bits:pos) = n
+
+(* Standard operators *)
+val add: a:uint64 -> b:uint64{v a + v b < reveal max_int} -> Tot uint64
+let add a b = uadd #n a b
+val add_mod: uint64 -> uint64 -> Tot uint64
+let add_mod a b = uadd_mod #n a b
+val sub: a:uint64 -> b:uint64{v a - v b >= reveal min_int} -> Tot uint64
+let sub a b = usub #n a b
+val sub_mod: uint64 -> uint64 -> Tot uint64
+let sub_mod a b = usub_mod #n a b
+val mul: a:uint64 -> b:uint64{v a * v b < reveal max_int} -> Tot uint64
+let mul a b = umul #n a b
+val mul_mod: a:uint64 -> b:uint64 -> Tot uint64
+let mul_mod a b = umul_mod #n a b
+val mul_wide: uint64 -> uint64 -> Tot uint128
+let mul_wide a b = umul_large #n a b
+val div: uint64 -> b:uint64{v b <> 0} -> Tot uint64
+let div a b = udiv #n a b
+val rem: uint64 -> b:uint64{v b <> 0} -> Tot uint64
+let rem a b = umod #n a b
+
+val logand: uint64 -> uint64 -> Tot uint64
+let logand a b = ulogand #n a b
+val logxor: uint64 -> uint64 -> Tot uint64
+let logxor a b = ulogxor #n a b
+val logor: uint64 -> uint64 -> Tot uint64
+let logor a b = ulogor #n a b
+val lognot: uint64 -> Tot uint64
+let lognot a = ulognot #n a
+
+val shift_left: uint64 -> nat -> Tot uint64
+let shift_left a s = ushift_left #n a s
+val shift_right: uint64 -> nat -> Tot uint64
+let shift_right a s = ushift_right #n a s
+
+let rotate_left a s = urotate_left #n a s
+let rotate_right a s = urotate_right #n a s
+
+val to_uint64: sint -> Tot uint64
+let to_uint64 s = to_usint n s
+
+let op_Less_Less = shift_left
+let op_Greater_Greater = shift_right
