examples/primitives/poly.fst
@@ -1,0 +1,391 @@
+(*--build-config
+  options:--admit_fsi FStar.Set --verify_module Poly1305 --z3timeout 10;
+  other-files:FStar.Classical.fst FStar.FunctionalExtensionality.fst FStar.Set.fsi seq.fsi FStar.Seq.fst FStar.SeqProperties.fst FStar.Heap.fst FStar.ST.fst FStar.All.fst FStar.Array.fst FStar.Ghost.fst axioms.fst intlib.fst lemmas.fst sint.fst FStar.UInt8.fst FStar.UInt63.fst sbuffer.fst parameters1305.fst bigint.fst bignum1305.fst FStar.SBytes.fst;
+  --*)
+
+(* Implementation of Chacha20 based on the rfc7539 *)
+(* Current issues:
+   - inplace modification of bytes ?
+   - automatization of the coercion between mathematical integers 'int' and concrete machine 
+   integers 'uint32', not only at compile time, but also in verification
+*)
+
+module Poly
+
+open FStar.Heap
+open FStar.Ghost
+open IntLib
+open Sint
+open FStar.UInt63
+open FStar.SBytes
+open SBuffer
+open Bigint
+open Parameters
+open Bignum
+
+(* Auxiliary lemmas and functions *)
+
+val max_value_increases: h:heap -> b:bigint{Live h b} -> n:pos -> m:pos{m>=n /\ m <= length b} -> Lemma
+  (maxValue h b n <= maxValue h b m)
+let rec max_value_increases h b n m =
+  match (m-n) with
+  | 0 -> () | _ -> max_value_increases h b n (m-1)
+
+val pow2_5_lemma: unit -> Lemma (requires (True)) (ensures (pow2 5 = 32))
+let pow2_5_lemma () = 
+  //admit();
+  ()
+
+opaque val gsatisfies_constraints_after_multiplication: h:heap -> b:bigint{Live h b /\ length b >= 2*norm_length-1 /\ maxValue h b (length b) <= norm_length * pow2 53} -> GLemma unit (requires (True))
+  (ensures (SatisfiesModuloConstraints h b)) []
+let gsatisfies_constraints_after_multiplication h b =
+  //admit();
+  max_value_increases h b (2*norm_length-1) (length b);
+  pow2_5_lemma ();
+  cut (maxValue h b (2*norm_length-1) * 6 <= 30 * pow2 53 /\ 30 * pow2 53 < pow2 5 * pow2 53);  
+  IntLibLemmas.pow2_exp 5 53;
+  IntLibLemmas.pow2_increases 63 58
+
+val satisfies_constraints_after_multiplication: h:heap -> b:bigint{Live h b /\ length b >= 2*norm_length-1 /\ maxValue h b (length b) <= norm_length * pow2 53} -> Lemma
+  (SatisfiesModuloConstraints h b)
+let satisfies_constraints_after_multiplication h b = 
+  coerce (requires (True))
+	 (ensures (SatisfiesModuloConstraints h b))
+	 (fun _ -> gsatisfies_constraints_after_multiplication h b)
+
+(* TODO *)
+opaque val aux_lemma': a:nat -> n:nat{n <= 32} -> GLemma unit (requires True) (ensures ((((a * pow2 (32 - n)) % pow2 63) % pow2 26) % pow2 (32 - n) = 0 )) []
+let aux_lemma' a n = 
+  admit();
+  if 32-n > 26 then (
+    IntLibLemmas.pow2_exp (32-n-26) 26;
+    IntLibLemmas.modulo_lemma (a * pow2 (32-n-26)) (pow2 26) )
+  else if 32 - n = 26 then 
+    IntLibLemmas.modulo_lemma a (pow2 26)
+  else ()
+
+opaque val gaux_lemma: x:uint63{v x < pow2 32} -> y:uint63{v y < pow2 32} -> n:nat{n >= 7 /\ n < 32} -> GLemma unit
+  (requires (True))
+  (ensures (IntLib.div (v x) (pow2 n) + (((v y * pow2 (32 - n)) % pow2 63) % pow2 26) < pow2 26)) []
+let gaux_lemma x y n =
+  //admit();
+  IntLibLemmas.div_pow2_inequality (v x) 32;
+  IntLibLemmas.pow2_increases 26 (32-n);
+  aux_lemma' (v y) n;
+  let a = IntLib.div (v x) (pow2 n) in
+  let b = ((v y * pow2 (32 - n)) % pow2 63) % pow2 26 in
+  let n1 = 26 in
+  let n2 = 32 - n in 
+  IntLibLemmas.div_positive (v x) (pow2 n); 
+  IntLibLemmas.pow2_disjoint_ranges a b n1 n2
+
+val aux_lemma: x:uint63{v x < pow2 32} -> y:uint63{v y < pow2 32} -> n:nat{n >= 7 /\ n < 32} -> Lemma
+  (requires (True))
+  (ensures (IntLib.div (v x) (pow2 n) + (((v y * pow2 (32 - n)) % pow2 63) % pow2 26) < pow2 26)) 
+let aux_lemma x y n =
+  coerce
+    (requires (True))
+    (ensures (IntLib.div (v x) (pow2 n) + (((v y * pow2 (32 - n)) % pow2 63) % pow2 26) < pow2 26)) 
+    (fun _ -> gaux_lemma x y n)
+
+opaque val gaux_lemma_1: x:uint63{v x < pow2 32} -> GLemma unit (requires (True)) (ensures (v (x ^>> 8) < pow2 24)) []
+let gaux_lemma_1 x = 
+  //admit();
+  IntLibLemmas.div_pow2_inequality (v x) 32  
+
+val aux_lemma_1: x:uint63{v x < pow2 32} -> Lemma (ensures (v (x ^>> 8) < pow2 24))
+let aux_lemma_1 x = 
+  coerce (requires (True)) (ensures (v (x ^>> 8) < pow2 24)) 
+    (fun _ -> gaux_lemma_1 x)
+    
+#reset-options
+
+opaque val gaux_lemma_2: b:bigint -> GLemma unit (requires (True)) (ensures ((arefs (only b)) = !{content b})) []
+let gaux_lemma_2 b = FStar.Set.lemma_equal_intro (arefs (only b)) !{content b};
+  cut (True /\ arefs (only b) = !{content b})
+
+val aux_lemma_2: b:bigint -> Lemma (requires (True)) (ensures ((arefs (only b)) = !{content b})) 
+let aux_lemma_2 b = 
+  coerce (requires (True)) (ensures ((arefs (only b)) = !{content b})) (fun _ -> gaux_lemma_2 b)
+
+val aux_lemma_3: h0:heap -> h1:heap -> b:bigint -> Lemma (requires (modifies (arefs (only b)) h0 h1))
+  (ensures (modifies !{content b} h0 h1))
+let aux_lemma_3 h0 h1 b = 
+  aux_lemma_2 b; ()
+
+#reset-options
+
+(* Poly1305 code *)
+
+(* Bigint to bytes serializing function *)
+val num_to_le_bytes: s:sbytes{length s >= 16} -> b:bigint{Disjoint b s} -> ST unit
+  (requires (fun h -> Norm h b /\ SBuffer.Live h s))
+  (ensures (fun h0 _ h1 -> SBuffer.Live h1 s /\ Modifies (only s) h0 h1))
+let num_to_le_bytes s b =
+  //admit();
+  let h0 = ST.get() in
+  let b0 = index b 0 in
+  let b1 = index b 1 in
+  let b2 = index b 2 in
+  let b3 = index b 3 in
+  let b4 = index b 4 in 
+  upd s 0 (FStar.UInt8.of_native_int b0);  // 0 
+  upd s 1 (FStar.UInt8.of_native_int (b0 ^>> 8)); //8
+  upd s 2 (FStar.UInt8.of_native_int (b0 ^>> 16)); //16
+  upd s 3 (FStar.UInt8.add_mod (FStar.UInt8.of_native_int (b0 ^>> 24)) // 24 
+			       (FStar.UInt8.of_native_int (b1 ^<< 2))); 
+  upd s 4 (FStar.UInt8.of_native_int (b1 ^>> 6)); // 32
+  upd s 5 (FStar.UInt8.of_native_int (b1 ^>> 14)); // 40
+  upd s 6 (FStar.UInt8.add_mod (FStar.UInt8.of_native_int (b1 ^>> 22)) 
+			       (FStar.UInt8.of_native_int (b2 ^<< 4))); // 48
+  upd s 7 (FStar.UInt8.of_native_int (b2 ^>> 4)); // 56
+  upd s 8 (FStar.UInt8.of_native_int (b2 ^>> 12)); // 64
+  upd s 9 (FStar.UInt8.add_mod (FStar.UInt8.of_native_int (b2 ^>> 20)) 
+			       (FStar.UInt8.of_native_int (b3 ^<< 6))); // 72
+  upd s 10 (FStar.UInt8.of_native_int (b3 ^>> 2)); // 80 
+  upd s 11 (FStar.UInt8.of_native_int (b3 ^>> 10)); // 88
+  let h = ST.get() in
+  cut (SBuffer.Live h s /\ Modifies (only s) h0 h); 
+  upd s 12 (FStar.UInt8.of_native_int (b3 ^>> 18)); // 96
+  upd s 13 (FStar.UInt8.of_native_int (b4)); // 104
+  upd s 14 (FStar.UInt8.of_native_int (b4 ^>> 8)); // 112 
+  upd s 15 (FStar.UInt8.of_native_int (b4 ^>> 16)); // 120 
+  ()
+
+#reset-options
+
+(* Bytes to bigint deserializing functions *)
+val le_bytes_to_num: b:bigint -> s:sbytes{length s = 16 /\ Disjoint b s} -> ST unit
+  (requires (fun h -> Live h b /\ SBuffer.Live h s))
+  (ensures (fun h0 _ h1 -> Norm h1 b /\ Modifies (only b) h0 h1  /\ v (get h1 b 4) < pow2 24))
+let le_bytes_to_num b s =
+  //admit();
+  IntLibLemmas.pow2_increases 63 26;
+  IntLibLemmas.pow2_increases 63 32;
+  IntLibLemmas.pow2_increases 26 24;
+  let mask_26 = FStar.UInt63.sub (FStar.UInt63.one ^<< 26) FStar.UInt63.one in 
+  cut (v mask_26 = v one * pow2 26 - v one /\ v one = 1); 
+  assert(v mask_26 = pow2 26 - 1); 
+  let s0 = sub s 0  4 in
+  let s1 = sub s 4  8 in
+  let s2 = sub s 8  12 in
+  let s3 = sub s 12 16 in
+  let n0 = of_uint32 (FStar.SBytes.uint32_of_sbytes s0) in 
+  let n1 = of_uint32 (FStar.SBytes.uint32_of_sbytes s1) in
+  let n2 = of_uint32 (FStar.SBytes.uint32_of_sbytes s2) in
+  let n3 = of_uint32 (FStar.SBytes.uint32_of_sbytes s3) in 
+  ulogand_lemma_4 #63 n0 26 mask_26;
+  ulogand_lemma_4 #63 (n1 ^<< 6) 26 mask_26; 
+  ulogand_lemma_4 #63 (n2 ^<< 12) 26 mask_26; 
+  ulogand_lemma_4 #63 (n3 ^<< 18) 26 mask_26;  
+  aux_lemma n0 n1 26; 
+  aux_lemma n1 n2 20;
+  aux_lemma n2 n3 14;  
+  aux_lemma_1 n3; 
+  let n0' = n0 ^& mask_26 in
+  let n1' = (n0 ^>> 26) ^+ ((n1 ^<< 6) ^& mask_26) in 
+  let n2' = (n1 ^>> 20) ^+ ((n2 ^<< 12) ^& mask_26) in
+  let n3' = (n2 ^>> 14) ^+ ((n3 ^<< 18) ^& mask_26) in 
+  let n4' = (n3 ^>> 8) in 
+  upd b 0 n0'; 
+  upd b 1 n1';
+  upd b 2 n2'; 
+  upd b 3 n3';
+  upd b 4 n4';
+  ()
+
+#reset-options
+
+(* Runs "Acc = ((Acc+block)*r) % p." *)
+val add_and_multiply: acc:bigint -> block:bigint{Disjoint acc block} -> r:bigint{Disjoint acc r /\ Disjoint block r} -> ST unit
+  (requires (fun h -> Norm h acc /\ Norm h block /\ Norm h r))
+  (ensures (fun h0 _ h1 -> Norm h0 acc /\ Norm h0 block /\ Norm h0 r /\ Norm h1 acc
+    /\ Modifies (only acc) h0 h1
+    /\ eval h1 acc norm_length % reveal prime = 
+    ((eval h0 acc norm_length + eval h0 block norm_length) * eval h0 r norm_length) % reveal prime))
+let add_and_multiply acc block r =
+  //admit();
+  let h0 = ST.get() in
+  fsum' acc block; 
+  let h1 = ST.get() in
+  let tmp = create #63 FStar.UInt63.zero (2*norm_length-1) in 
+  let h2 = ST.get() in 
+  cut (forall (i:nat). {:pattern (v (get h2 acc i))} i < norm_length ==> v (get h2 acc i) = v (get h1 acc i));
+  cut (forall (i:nat). {:pattern (v (get h1 acc i))} i < norm_length ==> v (get h1 acc i) = v (get h0 acc (i+0)) + v (get h0 block (i+0)));
+  cut (forall (i:nat). {:pattern (v (get h0 acc i))} i < norm_length ==> v (get h0 acc i) < pow2 26); 
+  cut (forall (i:nat). {:pattern (v (get h0 block i))} i < norm_length ==> v (get h0 block i) < pow2 26);
+  IntLibLemmas.pow2_doubles 26;
+  cut (forall (i:nat). {:pattern (v (get h2 acc i))} i < norm_length ==> v (get h2 acc i) < pow2 27);
+  cut (Bound27 h2 acc); 
+  eq_lemma h0 h2 r (only acc); 
+  cut (Null h2 tmp); 
+  multiplication tmp acc r; 
+  let h3 = ST.get() in
+  satisfies_constraints_after_multiplication h3 tmp;
+  modulo tmp; 
+  let h4 = ST.get() in
+  blit tmp 0 acc 0 norm_length;
+  let h5 = ST.get() in
+  cut (Modifies (only acc) h0 h5); 
+  cut (forall (i:nat). {:pattern (v (get h5 acc i))} i < norm_length ==> v (get h5 acc (0+i)) = v (get h4 tmp (0+i))); 
+  cut (Norm h5 acc); 
+  eval_eq_lemma h4 h5 tmp acc norm_length;
+  eval_eq_lemma h1 h2 acc acc norm_length;
+  eval_eq_lemma h0 h2 r r norm_length;
+  ()
+
+#reset-options
+
+val clamp: r:sbytes{length r = 16} -> ST unit
+  (requires (fun h -> SBuffer.Live h r))
+  (ensures (fun h0 _ h1 -> SBuffer.Live h1 r /\ Modifies (only r) h0 h1))
+let clamp r =
+  let mask_15 = FStar.UInt8.of_int 15 in
+  let mask_252 = FStar.UInt8.of_int 252 in
+  upd r 3 (index r 3 ^&  mask_15);
+  upd r 7 (index r 7 ^& mask_15);
+  upd r 11 (index r 11 ^& mask_15);
+  upd r 15 (index r 15 ^& mask_15);
+  upd r 4 (index r 4 ^& mask_252);
+  upd r 8 (index r 8 ^& mask_252);
+  upd r 12 (index r 12 ^& mask_252);
+  ()
+
+#reset-options
+
+val poly1305_step: msg:sbytes -> acc:bigint{Disjoint msg acc} -> 
+  bigint_r:bigint{Disjoint msg bigint_r /\ Disjoint acc bigint_r} -> ctr:nat{length msg >= 16 * ctr} ->
+  ST unit
+    (requires (fun h -> SBuffer.Live h msg /\ Norm h acc /\ Norm h bigint_r))
+    (ensures (fun h0 _ h1 -> SBuffer.Live h1 msg /\ Norm h1 acc /\ Norm h1 bigint_r
+      /\ Modifies (only acc) h0 h1))
+let rec poly1305_step msg acc r ctr =
+  //admit();
+  let h0 = ST.get() in
+  match ctr with
+  | 0 -> ()
+  | _ -> 
+    let n = sub msg 0 16 in
+    let msg = offset msg 16 in
+    //    let n, msg = FStar.SBytes.split msg 16 in 
+    let h = ST.get() in
+    let block = create #63 FStar.UInt63.zero norm_length in 
+    let h' = ST.get() in
+    le_bytes_to_num block n; 
+    let b4 = index block 4 in
+    IntLibLemmas.pow2_doubles 24; IntLibLemmas.pow2_increases 26 25;
+    IntLibLemmas.pow2_increases 63 26; 
+    upd block 4 (b4 ^+ (FStar.UInt63.one ^<< 24)); 
+    let h1 = ST.get() in
+    eq_lemma h0 h1 r (empty); 
+    eq_lemma h0 h1 acc empty;
+    add_and_multiply acc block r; 
+    let h2 = ST.get() in 
+    disjoint_only_lemma msg acc; 
+    eq_lemma h1 h2 r (only acc); 
+    eq_lemma h h2 msg (only acc); 
+    cut (Modifies (only acc) h0 h2); 
+    aux_lemma_2 acc;
+    cut (modifies (arefs (only acc)) h0 h2); 
+    aux_lemma_3 h0 h2 acc;
+    cut (modifies !{content acc} h0 h2); 
+    cut (SBuffer.Live h2 msg); 
+    poly1305_step msg acc r (ctr-1);
+    ()
+
+#reset-options
+
+val poly1305_last: msg:sbytes -> acc:bigint{Disjoint msg acc} -> 
+  bigint_r:bigint{Disjoint msg bigint_r /\ Disjoint acc bigint_r} -> len:nat{len <= length msg} ->
+  ST unit
+    (requires (fun h -> SBuffer.Live h msg /\ Norm h acc /\ Norm h bigint_r))
+    (ensures (fun h0 _ h1 -> SBuffer.Live h1 msg /\ Norm h1 acc /\ Norm h1 bigint_r
+      /\ Modifies (only acc) h0 h1))
+let poly1305_last msg acc r len =
+  //admit();
+  let h0 = ST.get() in
+  let l = len % 16 in
+  if l = 0 then ()
+  else (
+    let n = create FStar.UInt8.zero 16 in
+    blit msg (len - l) n 0 l; 
+    upd n l (FStar.UInt8.of_int 1);
+    let h1 = ST.get() in
+    let block = create #63 FStar.UInt63.zero norm_length in 
+    let h2 = ST.get() in
+    le_bytes_to_num block n; 
+    let b4 = index block 4 in
+    IntLibLemmas.pow2_doubles 24; IntLibLemmas.pow2_increases 26 25;
+    IntLibLemmas.pow2_increases 63 26; 
+    let h3 = ST.get() in
+    eq_lemma h0 h3 r (empty); 
+    eq_lemma h0 h3 acc empty;     
+    add_and_multiply acc block r;
+    let h4 = ST.get() in 
+    disjoint_only_lemma msg acc; 
+    eq_lemma h3 h4 r (only acc); 
+    eq_lemma h1 h4 msg (only acc); 
+    aux_lemma_2 acc;
+    aux_lemma_3 h0 h4 acc;
+    () )
+
+val poly1305_mac: hash:sbytes{length hash >= 16} -> msg:sbytes{Disjoint hash msg} -> 
+  len:nat{len <= length msg} -> key:sbytes{length key = 32 /\ Disjoint msg key /\ Disjoint hash key} -> 
+  ST unit
+    (requires (fun h -> SBuffer.Live h msg /\ SBuffer.Live h key /\ SBuffer.Live h hash))
+    (ensures (fun h0 _ h1 -> SBuffer.Live h1 hash /\ Modifies (only hash) h0 h1))
+let poly1305_mac hash msg len key =
+  //admit();
+  let h0 = ST.get() in
+  let r' = sub key 0 16 in
+  let s = sub key 16 32 in
+  //  let r',s = FStar.SBytes.split key 16 in 
+  let r = create FStar.UInt8.zero 16 in
+  blit r' 0 r 0 16;
+  let h0' = ST.get() in
+  clamp r; 
+  let h0'' = ST.get() in
+  let bigint_r = create #63 FStar.UInt63.zero norm_length in
+  let bigint_s = create #63 FStar.UInt63.zero norm_length in 
+  le_bytes_to_num bigint_r r; 
+  let h1 = ST.get() in
+  disjoint_only_lemma s r; 
+  le_bytes_to_num bigint_s s; 
+  let h2 = ST.get() in
+  cut (Modifies (only r) h0'' h2); 
+  let acc = create #63 FStar.UInt63.zero norm_length in 
+  let h2' = ST.get() in
+  let ctr = len / 16 in
+  let rest = len % 16 in 
+  eq_lemma h1 h2' bigint_r (only bigint_s); 
+  disjoint_only_lemma bigint_r bigint_s;
+  disjoint_only_lemma msg bigint_s;
+  admitP (Norm h2' bigint_r); 
+  admitP (SBuffer.Live h0' msg); 
+  disjoint_only_lemma msg r; 
+  cut (SBuffer.Live h0'' msg); 
+  poly1305_step msg acc bigint_r ctr; 
+  let h3 = ST.get() in
+  poly1305_last msg acc bigint_r len;
+  let h3' = ST.get() in
+  eq_lemma h2 h3' bigint_s empty; 
+  fsum' acc bigint_s; 
+  let h4 = ST.get() in
+  IntLibLemmas.pow2_doubles 26;
+  IntLibLemmas.pow2_increases 62 27; 
+  cut (forall (i:nat). {:pattern (v (get h3' acc i))} i < norm_length ==> v (get h3' acc i) < pow2 26); 
+  cut (forall (i:nat). {:pattern (v (get h3' bigint_s i))} i < norm_length ==> v (get h3' bigint_s i) < pow2 26); 
+  cut (forall (i:nat). {:pattern (v (get h4 acc i))} i < norm_length ==> v (get h4 acc i) = v (get h3' acc (i+0)) + v (get h3' bigint_s (i+0))); 
+  cut (forall (i:nat). {:pattern (v (get h4 acc i))} i < norm_length ==> v (get h4 acc i) < pow2 27);
+  cut (forall (i:nat). {:pattern (v (get h4 acc i))} i < norm_length ==> v (get h4 acc i) < pow2 63);
+  freduce_coefficients acc; 
+  disjoint_only_lemma hash r;  
+  let h5 = ST.get() in
+  disjoint_only_lemma hash bigint_r;  
+  disjoint_only_lemma hash bigint_s;  
+  disjoint_only_lemma hash acc;  
+  cut (SBuffer.Live h5 hash); 
+  num_to_le_bytes hash acc; 
+  let h6 = ST.get() in
+  cut (Modifies (only hash) h0 h6);
+  ()
