examples/primitives/sbuffer.fst
@@ -1,0 +1,279 @@
+(*--build-config
+  options:--admit_fsi FStar.Set --verify_module SBuffer --z3timeout 10;
+  other-files:FStar.Classical.fst FStar.PredicateExtensionality.fst FStar.Set.fsi seq.fsi FStar.Seq.fst FStar.SeqProperties.fst FStar.Heap.fst FStar.ST.fst FStar.All.fst FStar.Array.fst FStar.Ghost.fst axioms.fst intlib.fst sint.fst;
+  --*)
+
+module SBuffer
+
+open Sint
+open FStar.Seq
+open FStar.Heap
+open FStar.Array
+open FStar.Ghost
+
+(* Buffer general type *)
+private type buffer (t:pos) = {
+  content:array (usint t); // length "max_length"
+  idx:nat; 
+  length:nat; // idx + length <= max_length
+}
+
+type uint32s = buffer 32
+type uint8s = buffer 8
+type uint64s = buffer 64
+type uint128s = buffer 128
+
+(* Ghost spec-related functions *)
+val contains: heap -> #size:pos -> buffer size -> GTot bool
+let contains h #size (b:buffer size) = FStar.Heap.contains #(seq (usint size)) h b.content
+
+val sel: heap -> #size:pos -> buffer size -> GTot (seq (usint size))
+let sel h #size b = FStar.Heap.sel h b.content
+
+val max_length: heap -> #size:pos -> buffer size -> GTot nat
+let max_length h #size b = FStar.Seq.length (sel h b)
+
+val length: #size:pos -> buffer size -> GTot nat
+let length #size b = b.length
+
+val idx: #size:pos -> buffer size -> GTot nat
+let idx #size b = b.idx
+
+val content: #size:pos -> buffer size -> GTot (ref (seq (usint size)))
+let content #size b = b.content
+
+(* Liveness condition, necessary for any computation on the buffer *)
+type Live (h:heap) (#size:pos) (b:buffer size) = (contains h b /\ max_length h b >= length b + idx b)
+
+(* Memory separation condition, obtained either when getting a fresh buffer or
+   when getting disjoint subbuffers *)
+type Disjoint (#t:pos) (#t':pos) (b:buffer t) (b':buffer t') =
+  (FStar.Heap.Ref (b.content) <> FStar.Heap.Ref (b'.content))
+  \/ (FStar.Heap.Ref (b.content) = FStar.Heap.Ref (b'.content)
+     /\ (idx b + length b <= idx b' \/ idx b' + length b' <= idx b))
+
+(* Defines that sb is a subbuffer of b *)
+type SubBuffer (#t:pos) (sb:buffer t) (b:buffer t) =
+  (FStar.Heap.Ref b.content == FStar.Heap.Ref sb.content)
+  /\ idx sb >= idx b /\ idx b + length b >= idx sb + length sb
+
+(* Ghost getters for specs *)
+val getValue: h:heap -> #size:pos -> b:buffer size -> i:nat{i<max_length h b} -> GTot (usint size)
+let getValue h #size b i = Seq.index (sel h b) i
+
+val get: h:heap -> #size:pos -> b:buffer size{Live h b} -> i:nat{i<length b} -> GTot (usint size)
+let get h #size b i = Seq.index (sel h b) (idx b + i)
+
+(* Equality between buffers of sints *)
+opaque type Eq (#a:pos) (h0:heap) (b:buffer a) (h1:heap) (c:buffer a) =
+  Live h0 b /\ Live h1 c /\ length b = length c /\ 
+  (forall (i:nat). {:pattern (get h0 b i) \/ (get h1 c i)} i < length b ==> v (get h0 b i) = v (get h1 c i))
+
+(* Abstraction of buffers of any type *)
+type abuffer = | Buff: #t:pos -> b:buffer t -> abuffer
+
+let empty = FStar.Set.empty #abuffer
+let only #t b = FStar.Set.singleton (Buff #t b)
+val op_Plus_Plus: s:FStar.Set.set abuffer -> #t:pos -> b:buffer t -> Tot (s':FStar.Set.set abuffer{FStar.Set.subset s s' /\ FStar.Set.subset (only b) s'})
+let op_Plus_Plus set #t b = FStar.Set.union set (only b)
+
+(* Maps a set of buffer to the set of their references *)
+assume logic val arefs: FStar.Set.set abuffer -> Tot (FStar.Set.set aref)
+
+(** TODO: make it minimal & review **)
+assume Arefs1: forall (#size:pos) (b:buffer size) (s:FStar.Set.set abuffer). {:pattern (FStar.Set.mem (Ref (content b)) (arefs s))}
+	      FStar.Set.mem (Buff b) s ==> FStar.Set.mem (Ref (content b)) (arefs s)
+assume Arefs2: forall (s:FStar.Set.set abuffer) (s':FStar.Set.set abuffer). {:pattern (FStar.Set.subset s s')}
+	      FStar.Set.subset s s' ==> FStar.Set.subset (arefs s) (arefs s')
+assume Arefs3: arefs empty = FStar.Set.empty #aref
+assume Arefs4: forall (s1:FStar.Set.set abuffer) (s2:FStar.Set.set abuffer). {:pattern (FStar.Set.union s1 s2)}
+  FStar.Set.Equal (arefs (FStar.Set.union s1 s2)) (FStar.Set.union (arefs s1) (arefs s2))
+assume Arefs5: forall (#t:pos) (b:buffer t). {:pattern (arefs (FStar.Set.singleton (Buff b)))}
+  FStar.Set.Equal (arefs (FStar.Set.singleton (Buff b))) (FStar.Set.singleton (Ref (content b)))
+
+(* Specifies that a buffer is disjoint from a set of abstract buffers *)
+opaque type DisjointSet (#t:pos) (b:buffer t) (buffs:FStar.Set.set abuffer) =
+  (forall (#t':pos) (b':buffer t'). {:pattern (FStar.Set.mem (Buff b') buffs) \/ (Disjoint b b')} FStar.Set.mem (Buff b') buffs ==> Disjoint b b')
+
+(* Buffer specific modifies clause *)
+opaque type Modifies (buffs:FStar.Set.set abuffer) (h:heap) (h':heap) =
+  FStar.Heap.equal h' (FStar.Heap.concat h' (FStar.Heap.restrict h (FStar.Set.complement (arefs buffs))))
+  /\ (forall (#t:pos) (b:buffer t). {:pattern (DisjointSet b buffs)}
+				  (Live h b /\ DisjointSet b buffs) ==> Eq h b h' b)
+
+(** Lemmas; TODO: give better names, check triggers **)
+val disjoint_only_lemma: #t:pos -> b:buffer t -> #t':pos -> b':buffer t' -> Lemma
+  (requires (Disjoint b b'))
+  (ensures (DisjointSet b (only b')))
+let disjoint_only_lemma #t b #t' b' = ()  
+
+val eq_lemma: h0:heap -> h1:heap -> #size:pos -> a:buffer size -> mods:FStar.Set.set abuffer ->
+  Lemma (requires (Live h0 a /\ DisjointSet a mods /\ Modifies mods h0 h1))
+	(ensures (Eq h0 a h1 a))
+	[SMTPatT (DisjointSet a mods); SMTPatT (Modifies mods h0 h1)]
+let eq_lemma h0 h1 #size a mods = ()
+
+val modifies_transitivity_lemma: mods: FStar.Set.set abuffer -> h0:heap -> h1:heap -> h2:heap -> 
+  Lemma (requires (Modifies mods h0 h1 /\ Modifies mods h1 h2))
+	(ensures (Modifies mods h0 h2))
+	[SMTPatT (Modifies mods h0 h1); SMTPatT (Modifies mods h1 h2)]
+let modifies_transitivity_lemma mods h0 h1 h2 = ()
+
+val modifies_subset_lemma: mods:FStar.Set.set abuffer -> submods:FStar.Set.set abuffer ->  h0:heap -> 
+  h1:heap -> Lemma 
+    (requires (FStar.Set.subset submods mods /\ Modifies submods h0 h1))
+    (ensures (Modifies mods h0 h1))
+    [SMTPatT (Modifies submods h0 h1); SMTPat (FStar.Set.subset submods mods)]
+let modifies_subset_lemma mods submods h0 h1 = 
+  cut (modifies (arefs mods) h0 h1);
+  cut (forall (#t:pos) (b:buffer t). (Live h0 b /\ DisjointSet b mods) ==> (Live h0 b /\ DisjointSet b submods) ==> Eq h0 b h1 b)
+
+val modifies_empty_lemma: h:heap -> Lemma (requires (True)) (ensures (Modifies empty h h))
+let modifies_empty_lemma h = ()
+
+val modifies_fresh_lemma: h0:heap -> h1:heap -> mods:FStar.Set.set abuffer -> #size:pos -> 
+  b:buffer size -> Lemma 
+    (requires (not(contains h0 b) /\ modifies (arefs (mods ++ b)) h0 h1))
+    (ensures (modifies (arefs mods) h0 h1))
+let modifies_fresh_lemma h0 h1 mods #size b = ()
+
+val modifies_fresh: h0:heap -> h1:heap -> mods:FStar.Set.set abuffer -> #size:pos -> b:buffer size ->
+  Lemma (requires (not(contains h0 b) /\ Modifies (mods ++ b) h0 h1))
+	(ensures (Modifies (mods) h0 h1))
+	[SMTPat (not(contains h0 b)); SMTPatT (Modifies (mods ++ b) h0 h1)]
+let modifies_fresh h0 h1 mods #size b =
+  cut (FStar.Set.mem (Buff b) (mods ++ b) /\ True); 
+  cut (forall (#t:pos) (s:buffer t). (DisjointSet s mods /\ Disjoint s b) ==> DisjointSet s (mods ++ b))
+
+val modifies_subbuffer_lemma: h0:heap -> h1:heap -> mods:FStar.Set.set abuffer -> #size:pos ->
+  b:buffer size -> b':buffer size -> Lemma 
+    (requires (Modifies (mods ++ b) h0 h1 /\ SubBuffer #size b b'))
+    (ensures (Modifies (mods ++ b') h0 h1))
+    [SMTPatT (Modifies (mods ++ b) h0 h1); SMTPatT (SubBuffer #size b b')]
+let modifies_subbuffer_lemma h0 h1 mods #size b b' =
+  cut (FStar.Set.mem (Buff b') (mods ++ b') /\ True); 
+  cut (forall (#t:pos) (s:buffer t). (DisjointSet s mods /\ Disjoint s b) ==> DisjointSet s (mods ++ b))
+
+(* Equality between fragments of buffers *)
+opaque type EqSub (#t:pos) (ha:heap) (a:buffer t) (a_idx:nat) (hb:heap) (b:buffer t) (b_idx:nat) (len:nat) =
+  (Live ha a) /\ (Live hb b) /\ (length a >= a_idx + len) /\ (length b >= b_idx + len)
+  /\ (forall (i:nat). {:pattern (get ha a (a_idx+i)) \/ (get hb b (b_idx+i))} i < len ==> v (get ha a (a_idx+i)) = v (get hb b (b_idx+i)))
+
+(* Specifies an atomic update to a buffer *)
+opaque type AtomicUpdate (#a:pos) (h0:heap) (h1:heap) (b:buffer a) (n:nat) (z:usint a) =
+  Live h0 b /\ Live h1 b /\ n < length b /\ v (get h1 b n) = v z /\ max_length h1 b = max_length h0 b 
+  /\ (forall (i:nat). {:pattern (get h1 b i)} (i < length b /\ i <> n) ==> v (get h1 b i) = v (get h0 b i))
+  /\ Modifies (only b) h0 h1
+  
+(** TODO: merge with EqSub ? **)
+opaque type CopyOf (#t:pos) (h:heap) (a:buffer t) (idx_a:nat) (b:buffer t) (idx_b:nat) (ctr:nat) (len:nat) =
+  idx_a <= length a /\ idx_b <= length b /\ idx_a+len <= length a /\ idx_b+len <= length b /\ ctr <= len /\
+  Live h a /\ Live h b /\ 
+  (forall (i:nat). {:pattern (get h a (idx_a+i)) \/ (get h b (idx_b+i))} (i >= ctr /\ i < len) ==>
+    v (get h a (idx_a+i)) = v (get h b (idx_b+i)))
+
+(** Concrete getters and setters **)
+
+val create: #a:pos -> init:usint a -> len:pos -> ST (buffer a)
+  (requires (fun h -> True))
+  (ensures (fun h0 b h1 ->
+    not(contains h0 b) /\ Live h1 b /\ idx b = 0 /\ length b = len 
+    /\ Modifies empty h0 h1
+    /\ (forall (i:nat). {:pattern (v (get h1 b i))} i < len ==> 
+	v (get h1 b i) = v init)))
+let create #a init len =
+  let content = FStar.Array.create len init in 
+  {content = content; idx = 0; length = len}
+
+val index: #a:pos -> b:buffer a -> n:nat{n < length b} -> ST (usint a)
+  (requires (fun h -> Live h b))
+  (ensures (fun h0 z h1 -> Live h0 b /\ (h1 == h0) /\ (v z == v (get h0 b n))))
+let index #a b n = Array.index b.content (b.idx+n)
+
+val upd: #a:pos ->  b:buffer a -> n:nat{n < length b} -> v:usint a -> ST unit
+  (requires (fun h -> Live h b))
+  (ensures (fun h0 _ h1 -> AtomicUpdate h0 h1 b n v))
+let upd #a b n z =
+  FStar.Array.upd b.content (b.idx+n) z; 
+  cut (FStar.Set.mem (Buff b) (only b) /\ True)
+
+val sub: #a:pos -> b:buffer a -> i:nat -> len:nat{len <= length b /\ i + len <= length b} -> 
+  ST (buffer a)
+    (requires (fun h -> Live h b))
+    (ensures (fun h0 b' h1 -> content b = content b' /\ idx b' = idx b + i /\ length b' = len /\ (h0 == h1)))
+let sub #a b i len =
+  {content = b.content; idx = i+b.idx; length = len}
+
+private val blit_aux: #t:pos -> a:buffer t -> idx_a:nat{idx_a <= length a} -> b:buffer t{Disjoint a b} -> 
+  idx_b:nat{idx_b <= length b} -> len:nat{idx_a+len <= length a /\ idx_b+len <= length b} ->
+  ctr:nat{ctr<=len} -> ST unit
+    (requires (fun h -> CopyOf h a idx_a b idx_b ctr len))
+    (ensures (fun h0 _ h1 -> CopyOf h0 a idx_a b idx_b ctr len 
+      /\ CopyOf h1 a idx_a b idx_b 0 len /\ Modifies (only b) h0 h1
+      /\ (forall (i:nat). {:pattern (v (get h1 b i))} ((i >= idx_b + ctr /\ i < length b) \/ i < idx_b) ==> v (get h1 b i) = v (get h0 b i))))
+let rec blit_aux #t a idx_a b idx_b len ctr =
+  let h0 = ST.get() in
+  match ctr with
+  | 0 -> ()
+  | _  -> let i = ctr-1 in
+    let ai = index a (idx_a+i) in
+    upd b (idx_b+i) ai; 
+    let h1 = ST.get() in 
+    eq_lemma h0 h1 a (only b); 
+    blit_aux a idx_a b idx_b len i
+
+val blit: #t:pos -> a:buffer t -> idx_a:nat{idx_a <= length a} -> b:buffer t{Disjoint a b} -> 
+  idx_b:nat{idx_b <= length b} -> len:nat{idx_a+len <= length a /\ idx_b+len <= length b} -> ST unit
+    (requires (fun h -> Live h a /\ Live h b))
+    (ensures (fun h0 _ h1 -> Live h0 b 
+      /\ CopyOf h1 a idx_a b idx_b 0 len
+      /\ (forall (i:nat). {:pattern (v (get h1 b i))} ((i >= idx_b + len /\ i < length b) \/ i < idx_b) ==> v (get h1 b i) = v (get h0 b i))
+      /\ Modifies (only b) h0 h1))
+let blit #t a idx_a b idx_b len = blit_aux a idx_a b idx_b len len
+
+val split: #t:pos -> a:buffer t -> i:nat{i <= length a} -> ST (buffer t * buffer t)
+    (requires (fun h -> Live h a))
+    (ensures (fun h0 b h1 -> Live h1 (fst b) /\ Live h1 (snd b) /\ h1 == h0 /\ idx (fst b) = idx a 
+      /\ idx (snd b) = idx a + i /\ length (fst b) = i /\ length (snd b) = length a - i 
+      /\ Disjoint (fst b) (snd b)  /\ content (fst b) = content a /\ content (snd b) = content a))
+let split #t a i = 
+  let a1 = sub a 0 i in let a2 = sub a i (a.length - i) in a1, a2  
+
+val offset: #t:pos -> a:buffer t -> i:nat{i <= length a} -> ST (buffer t)
+  (requires (fun h -> Live h a))
+  (ensures (fun h0 a' h1 -> h0 == h1 /\ content a' = content a /\ idx a' = idx a + i /\ length a' = length a - i))
+let offset #t a i = {content = a.content; idx = i+a.idx; length = a.length - i}
+
+private val of_seq_aux: #a:pos -> s:seq (usint a) -> l:pos{l = FStar.Seq.length s} -> ctr:nat{ ctr <= l} -> b:buffer a{idx b = 0 /\ length b = l} -> ST unit
+    (requires (fun h -> Live h b))
+    (ensures (fun h0 _ h1 -> Live h0 b /\ Live h1 b 
+      /\ (forall (i:nat). {:pattern (v (get h1 b i))} i < ctr ==> v (get h1 b i) = v (FStar.Seq.index s i))
+      /\ (forall (i:nat). {:pattern (v (get h1 b i))} i >= ctr /\ i < length b ==> v (get h1 b i) = v (get h0 b i))))
+let rec of_seq_aux #size s l ctr b =
+  let h0 = ST.get() in
+  match ctr with
+  | 0 -> ()
+  | _ -> let j = ctr - 1 in 
+         upd b j (FStar.Seq.index s j); 
+	 of_seq_aux s l j b	 
+
+val of_seq: #a:pos -> s:seq (usint a) -> l:pos{l = FStar.Seq.length s} -> ST (buffer a)
+  (requires (fun h -> True))
+  (ensures (fun h0 b h1 -> idx b = 0 /\ length b = l /\ not(contains h0 b) /\ Live h1 b
+    /\ (forall (i:nat). {:pattern (v (get h1 b i))} i < l ==> v (get h1 b i) = v (FStar.Seq.index s i)) ))
+let of_seq #size s l =
+  let init = FStar.Seq.index s 0 in
+  let b = create #size init l in 
+  of_seq_aux s l l b; 
+  b
+
+val copy: #a:pos ->  b:buffer a -> l:pos{length b >= l} -> ST (buffer a)
+  (requires (fun h -> Live h b))
+  (ensures (fun h0 b' h1 -> not(contains h0 b') /\ contains h1 b' /\ idx b' = 0 
+	      /\ length b' = l /\ CopyOf #a h1 b 0 b' 0 0 l
+	      /\ Modifies empty h0 h1))
+let copy #size b l =
+  let init = index b 0 in 
+  let b' = create init l in 
+  blit b 0 b' 0 l; 
+  b'
